examples/pseudo_bool/cp_encoding/array/cpProgScript.sml
@@ -113,11 +113,17 @@ val res = translate sexp_linear_dispatch_def;
 (* lex *)
 val res = translate sexp_lex_dispatch_def;
 
-(* extensional (table) *)
+(* extensional (table, regular) *)
 val res = translate sexp_table_entry_def;
 val res = translate sexp_table_row_def;
 val res = translate sexp_table_rows_def;
 val res = translate sexp_table_body_def;
+val res = translate sexp_num_def;
+val res = translate sexp_num_list_def;
+val res = translate sexp_reg_edge_def;
+val res = translate sexp_reg_edges_def;
+val res = translate sexp_reg_trans_def;
+val res = translate sexp_regular_body_def;
 val res = translate sexp_extensional_dispatch_def;
 
 (* array *)
@@ -160,6 +166,7 @@ val res = translate sexp_misc_dispatch_def;
 
 (* scheduling *)
 val res = translate sexp_disjunctive_body_def;
+val res = translate sexp_disjunctive2d_body_def;
 val res = translate sexp_cumulative_body_def;
 val res = translate sexp_scheduling_dispatch_def;
 
@@ -512,6 +519,36 @@ val res = translate cp_to_ilp_extensionalTheory.cencode_full_eqs_def;
 val res = translate cp_to_ilp_extensionalTheory.creify_tuple_eq_def;
 val res = translate cp_to_ilp_extensionalTheory.creify_tuple_eqs_def;
 val res = translate cp_to_ilp_extensionalTheory.cencode_table_def;
+
+(* regular *)
+
+(* the translated EL precondition holds for any in-bounds index *)
+Theorem el_side_imp[local]:
+  ∀xs n. n < LENGTH xs ⇒ el_side n xs
+Proof
+  Induct>>rw[Once npbc_arrayProgTheory.el_side_def]
+QED
+
+val res = translate cpTheory.nfa_edges_def;
+
+Theorem nfa_edges_side:
+  nfa_edges_side trans q ⇔ T
+Proof
+  rw[fetch "-" "nfa_edges_side_def"]>>metis_tac[el_side_imp]
+QED
+
+val _ = update_precondition nfa_edges_side;
+
+val res = translate cp_to_ilp_extensionalTheory.reg_state_def;
+val res = translate cp_to_ilp_extensionalTheory.state_idx_row;
+val res = translate cp_to_ilp_extensionalTheory.state_idx_def;
+val res = translate cp_to_ilp_extensionalTheory.start_state_def;
+val res = translate cp_to_ilp_extensionalTheory.accept_state_def;
+val res = translate cp_to_ilp_extensionalTheory.reg_targets_def;
+val res = translate cp_to_ilp_extensionalTheory.reg_frame_def;
+val res = translate cp_to_ilp_extensionalTheory.reg_trans_def;
+val res = translate cp_to_ilp_extensionalTheory.reg_eq_pairs_def;
+val res = translate cp_to_ilp_extensionalTheory.cencode_regular_def;
 val res = translate cp_to_ilp_extensionalTheory.cencode_extensional_constr_def;
 
 (* cp_to_ilp_logical *)
@@ -606,6 +643,13 @@ val res = translate cp_to_ilp_miscTheory.cencode_knapsack_def;
 val res = translate cp_to_ilp_miscTheory.cencode_misc_constr_def;
 
 (* cp_to_ilp_scheduling *)
+val res = translate cp_to_ilp_schedulingTheory.disj_before_def;
+val res = translate cp_to_ilp_schedulingTheory.disj_zero_def;
+val res = translate cp_to_ilp_schedulingTheory.zsize_inactive_def;
+val res = translate cp_to_ilp_schedulingTheory.zsize_lit_def;
+val res = translate cp_to_ilp_schedulingTheory.mk_before_links_def;
+val res = translate cp_to_ilp_schedulingTheory.mk_zero_links_def;
+val res = translate cp_to_ilp_schedulingTheory.mk_sep_clauses_def;
 val res = translate cp_to_ilp_schedulingTheory.cencode_disjunctive_def;
 val res = translate cp_to_ilp_schedulingTheory.cencode_disjunctive2d_def;
 val res = translate cp_to_ilp_schedulingTheory.cencode_cumulative_def;
